src/impl/TLS13.Impl.Server.Driver.fst
@@ -10,6 +10,7 @@ module BL = TLS13.Impl.Server.Driver.BufferedLifecycle
 module BH = TLS13.Impl.Server.Driver.BufferedHandshake
 module BLoc = TLS13.Impl.Server.Driver.BufferedLocal
 module BN = TLS13.Impl.Server.Driver.BufferedNetwork
+module BW = TLS13.Impl.Server.Driver.BufferedWorkflow
 module CI = Common.ChannelImplementation
 module CPI = Common.ProtocolImplementation
 module CTypes = TLS13.Impl.CanonicalTypes
