Makefile
@@ -527,6 +527,7 @@ SERVER_DRIVER_MODULES = \
   TLS13.Impl.Server.Driver.BufferedLifecycle \
   TLS13.Impl.Server.Driver.BufferedHandshake \
   TLS13.Impl.Server.Driver.BufferedLocal \
+  TLS13.Impl.Server.Driver.BufferedWorkflow \
   TLS13.Impl.Server.Driver.Local \
   TLS13.Impl.Server.Driver.Handshake \
   TLS13.Impl.Server.Driver
